StoreO OFE

src/Iris/Algebra/Heap.lean
@@ -7,21 +7,76 @@ Authors: Markus de Medeiros
 import Iris.Algebra.CMRA
 import Iris.Algebra.OFE
 
-/- # Datatype and CMRA for a generic heap-like structure -/
+open Iris
+
+/- # Datatype and CMRA for a generic heap-like structure.
+
+Like FunLike in Mathlib, but not exactly the same, since the type must also be able to be updated. -/
 
 open Classical in
 noncomputable def fset {K V : Type _} (f : K → V) (k : K) (v : V) : K → V :=
   fun k' => if (k = k') then v else f k'
 
 /-- `T` can store and retrieve keys and values. -/
-class StoreLike (T K V : Type _) where
+class StoreLike (T : Type _) (K V : outParam (Type _)) where
   get : T → K → V
   set : T → K → V → T
+  of_fun : (K → V) → T
 export StoreLike (get set)
 
 /-- `T`'s store and retrieve operations behave like a classical store. -/
-class Store (T K V : Type _) extends StoreLike T K V where
+class Store (T : Type _) (K V : outParam (Type _)) extends StoreLike T K V where
   get_set {t k v} : get (set t k v) = fset (get t : K → V) k v
+  /-- One-sided inverse between get and of_fun. The other direction does not need to hold. -/
+  of_fun_get {f} : get (of_fun f) = f
+
+class Alloc (T : Type _) (K : outParam (Type _)) where
+  fresh : T → K
 
 /-- A type is HeapLike when it behaves like store for Optional values -/
-class abbrev HeapLike (T K V : Type _) := StoreLike T K (Option V)
+class Heap (T : Type _) (K V : outParam (Type _)) extends StoreLike T K (Option V), Alloc T K where
+  fresh_get {t} : get t (fresh t) = none
+
+
+namespace Store
+variable {T K V : Type _} [Store T K V]
+
+theorem get_set_ne {m : T} (H : k ≠ k') : get (set m k v) k' = get m k' := by
+  rw [get_set]; unfold fset; rw [if_neg H]
+
+theorem get_set_eq {m : T} (H : k = k') : get (set m k v) k' = v := by
+  rw [get_set]; unfold fset; rw [if_pos H]
+
+end Store
+
+
+/-- Wrapper type for functions with the Store OFE -/
+structure StoreO (T : Type _) where car : T
+
+section algebra
+
+open OFE
+
+/-- The OFE on StoreO is the discrete function OFE on it's .get function. -/
+instance StoreO_OFE {T K V : Type _} [StoreLike T K V] [OFE V] : OFE (StoreO T) where
+  Equiv s0 s1  := StoreLike.get s0.1 ≡ StoreLike.get s1.1
+  Dist n s0 s1 := StoreLike.get s0.1 ≡{n}≡ StoreLike.get s1.1
+  dist_eqv     := ⟨fun _ => .of_eq rfl, (·.symm), (·.trans ·)⟩
+  equiv_dist   := equiv_dist
+  dist_lt      := dist_lt
+
+def StoreO.toMap {T K V : Type _} [StoreLike T K V] [OFE V] : (StoreO T) -n> (K → V) where
+  f x := StoreLike.get <| StoreO.car x
+  ne.1 {_ _ _} H k := H k
+
+def StoreO.ofMap {T K V : Type _} [Store T K V] [OFE V] : (K → V) -n> (StoreO T) where
+  f x := StoreO.mk <| StoreLike.of_fun x
+  ne.1 {_ _ _} H k := by rw [Store.of_fun_get, Store.of_fun_get]; exact H k
+
+instance StoreO_COFE {T K V : Type _} [Store T K V] [COFE V] : COFE (StoreO T) where
+  compl c := ⟨StoreLike.of_fun <| COFE.compl <| c.map StoreO.toMap⟩
+  conv_compl {n c} k := by
+    rw [Store.of_fun_get]
+    exact COFE.conv_compl (c := Chain.map StoreO.toMap c) k
+
+end algebra
